feat: add error, let and constants
Developed against the PIR from plutus-cert, so it can actually handle the more complicated constant type already, it's just a hassle to import in a standalone project so I use the simpler definition for now. In the meantime I can figure out if it is possible for to figure out which show instance to use without explicitly matching the constant

src/PIR.v
@@ -2,10 +2,25 @@ From Coq Require Import String.
 #[local] Open Scope string_scope.
 (* Restricted version of the AST from plutus-cert *)
 
+Inductive recursivity := NonRec | Rec.
+
+Inductive strictness := NonStrict | Strict.
+
 Inductive DefaultUni : Type :=
-  | DefaultUniInteger
-  | DefaultUniBool
-.
+    | DefaultUniInteger
+    | DefaultUniByteString
+    | DefaultUniString
+    | DefaultUniUnit
+    | DefaultUniBool
+    | DefaultUniProtoList
+    | DefaultUniProtoPair
+    | DefaultUniData
+    | DefaultUniBLS12_381_G1_Element
+    | DefaultUniBLS12_381_G2_Element
+    | DefaultUniBLS12_381_MlResult
+
+    | DefaultUniApply : DefaultUni -> DefaultUni -> DefaultUni
+    .
 
 Inductive DefaultFun :=
   | AddInteger
@@ -20,16 +35,28 @@ Inductive DefaultFun :=
   | LessThanEqualsInteger
 .
 
+Definition name := string.
+Definition tyname := string.
+Definition binderName := string.
+Definition binderTyname := string.
+
 Inductive ty :=
   | Ty_Builtin : DefaultUni -> ty
   | Ty_Fun : ty -> ty -> ty
 .
 
+Inductive vdecl := VarDecl : binderName -> ty -> vdecl.
+
 (* for now, we trust the string representing a value is correct *)
 Inductive term :=
+  | Let      : recursivity -> list binding -> term -> term
   | Var      : string -> term
   | LamAbs   : string -> ty -> term -> term
-  | App      : term -> term -> term
+  | Apply    : term -> term -> term
   | Builtin  : DefaultFun -> term
   | Constant : ty -> string -> term
+  | Error    : ty -> term
+
+with binding :=
+  | TermBind : strictness -> vdecl -> term -> binding
 .
