src/Printer.v
@@ -1,10 +1,15 @@
+From Coq Require Import String BinInt List.
 
-Require Import Strings.String.
-Open Scope string.
-
+(* printing functionality *)
 From SimpleIO Require Import SimpleIO.
-From Coq Require Import String.
-#[local] Open Scope string_scope.
+(* afaik Coq has no builtin string conversion methods
+for its primitive types so we import the ones from QuickChick *)
+From QuickChick Require Import Show.
+Import ShowFunctions.
+
+Import ListNotations.
+Local Open Scope string_scope.
+Local Open Scope Z_scope.
 
 From PPIR Require Import PIR.
 
@@ -16,15 +21,75 @@ Definition brackets : string -> string :=
   fun x => "[" ++ x ++ "]"
 .
 
-Definition pretty_print_DefaultUni (D : DefaultUni) : string :=
-  match D with
+#[global]
+Instance ShowRec : Show recursivity :=
+{|
+  show rec := match rec with
+  | NonRec => "nonrec"
+  | Rec    => "rec" 
+  end
+|}.
+
+#[global]
+Instance ShowStrictness : Show strictness :=
+{|
+  show st := match st with
+  | NonStrict => "nonstrict"
+  | Strict    => "strict" 
+  end
+|}.
+
+Fixpoint show_DefaultUni (U : DefaultUni) : string :=
+  match U with
   | DefaultUniInteger => "integer"
+  | DefaultUniByteString => "bytestring"
+  | DefaultUniString => "string"
+  | DefaultUniUnit => "unit"
   | DefaultUniBool => "bool"
+  | DefaultUniProtoList => "list" (* is this correct? *)
+  | DefaultUniProtoPair => "pair"
+  | DefaultUniData => "data"
+  | DefaultUniBLS12_381_G1_Element => "bls12_381_G1_element"
+  | DefaultUniBLS12_381_G2_Element => "bls12_381_G2_element"
+  | DefaultUniBLS12_381_MlResult => "bls12_381_mlresult"
+
+  | DefaultUniApply U1 U2 =>
+      parens ((show_DefaultUni U1) ++ " " ++ (show_DefaultUni U2)) 
   end
 .
 
-Definition pretty_print_DefaultFun (F : DefaultFun) : string :=
-  match F with
+#[global]
+Instance ShowDefaultUni : Show DefaultUni :=
+{|
+  show := show_DefaultUni
+|}.
+
+(* Definition show_Constant (cst : constant) : string :=
+  let val := match cst with
+  (* | ValueOf uni val => "con " ++ show uni ++ " " ++ show val end in (* possible to infer show? *) *)
+  | ValueOf DefaultUniInteger z => show_Z z
+  | ValueOf DefaultUniByteString bs => "NotImplemented:bs"
+  | ValueOf DefaultUniString str => "NotImplemented:str"
+  | ValueOf DefaultUniUnit u => "unit"
+  | ValueOf DefaultUniData d => "NotImplemented:data"
+  | ValueOf DefaultUniBLS12_381_G1_Element z => show_Z z
+  | ValueOf DefaultUniBLS12_381_G2_Element z => show_Z z
+  | ValueOf DefaultUniBLS12_381_MlResult z => show_Z z
+  | ValueOf DefaultUniBool b => show_bool b
+  | _ => "UnknownUniverse" end in
+  "con " ++ match cst with (ValueOf uni _) => show uni end ++ " " ++ val
+. *)
+
+(* #[global]
+Instance ShowConstant : Show constant :=
+{|
+  show := show_Constant
+|}. *)
+
+#[global]
+Instance ShowDefaultFun : Show DefaultFun :=
+{|
+  show df := match df with
   | AddInteger => "addInteger"
   | SubtractInteger => "subtractInteger"
   | MultiplyInteger => "multiplyInteger"
@@ -36,29 +101,66 @@ Definition pretty_print_DefaultFun (F : DefaultFun) : string :=
   | LessThanInteger => "lessThanInteger"
   | LessThanEqualsInteger => "lessThanEqualsInteger"
   end
-.
+|}.
 
-Definition pretty_print_ty (T : ty) : string :=
+Fixpoint show_ty (T : ty) : string :=
   match T with
-  | Ty_Builtin D => "con " ++ pretty_print_DefaultUni D
-  | Ty_Fun T1 T2 => "ERROR: undefined"
+  | Ty_Builtin D => "con " ++ show D
+  | Ty_Fun T1 T2 => "fun " ++ (show_ty T1) ++ " " ++ (show_ty T2)
   end
 .
 
-Fixpoint pretty_print' (t : term) : string :=
+#[global]
+Instance ShowTy : Show ty :=
+{|
+  show := show_ty
+|}.
+
+Definition show_vdecl (vd : vdecl) : string :=
+  match vd with
+  | VarDecl bn T => "vardecl " ++ bn ++ " " ++ parens (show T) end
+.
+
+#[global]
+Instance ShowVDecl : Show vdecl :=
+{|
+  show := show_vdecl
+|}.
+
+Fixpoint show_term (t : term) : string :=
   match t with
+  | Let rec bds t => parens (
+      "let " ++ parens (show rec) ++ " "
+      ++ string_concat (map show_binding bds)
+      ++ " " ++ show_term t)
   | Var x => x
   | LamAbs x T t => parens (
       "lam " ++ x ++ " "
-      ++ parens (pretty_print_ty T)
-      ++ " " ++ (pretty_print' t)
-    )
-  | App t1 t2 => brackets (
-    (pretty_print' t1) ++ " " 
-    ++ pretty_print' t2)
-  | Builtin def => parens ("builtin " ++ (pretty_print_DefaultFun def))
-  | Constant T v => parens ((pretty_print_ty T) ++ " " ++ v)
+      ++ parens (show T)
+      ++ " " ++ show_term t)
+  | Apply t1 t2 => brackets ((show_term t1) ++ " " ++ show_term t2)
+  | Builtin def => parens ("builtin " ++ (show def))
+  | Error T => parens ("error " ++ show T)
+  (* | Constant cst => parens (show cst) *)
+  | Constant T cst => parens (show T) ++ " " ++ parens cst
   end
+
+with show_binding (b : binding) : string := 
+  match b with
+  | TermBind strc vdecl t => parens (
+      "termbind " ++ parens (show strc)
+      ++ " " ++ parens (show vdecl)
+      ++ " " ++ show_term t) end
+.
+
+#[global]
+Instance ShowTerm : Show term :=
+{|
+  show := show_term
+|}.
+
+Definition print_as_program (t : term) :=
+  parens ("program" ++ " " ++ "1.1.0" ++ " " ++ show t)
 .
 
 (* λ(x : Int) . x *)
@@ -68,23 +170,30 @@ Definition identity_ast : term :=
 
 (* (λ(x : Int) . (λ(y : Int). x + y)) 1 *)
 Definition plus_ast : term :=
-  (App
+  (Apply
     (LamAbs "x" (Ty_Builtin DefaultUniInteger)
       (LamAbs "y" (Ty_Builtin DefaultUniInteger)
-        (App (App (Builtin AddInteger) (Var "x")) (Var "y"))))
+        (Apply (Apply (Builtin AddInteger) (Var "x")) (Var "y"))))
   (Constant (Ty_Builtin DefaultUniInteger) "1")).
 
-Definition print_as_program (t : term) :=
-  parens ("program" ++ " " ++ "1.1.0" ++ " " ++
-    (pretty_print' t)
-  )
-.
+Definition let_ast : term :=
+  (Let NonRec 
+    [(TermBind Strict 
+        (VarDecl "x" (Ty_Builtin DefaultUniInteger)) 
+        (Error (Ty_Builtin DefaultUniInteger)))]
+    (Apply 
+      (Apply (Builtin EqualsInteger)
+             (Apply 
+                (Apply (Builtin AddInteger) (Constant (Ty_Builtin DefaultUniInteger) "10"))
+                (Var "x")))
+      (Constant (Ty_Builtin DefaultUniInteger) "5"))).
+
 Import IO.Notations.
 
-Definition test_file := plus_ast.
+Definition test_file := let_ast.
 Eval cbv in (print_as_program test_file).
 Definition main : IO unit :=
-  chan <- open_out "test.pir" ;;
+  chan <- open_out "printing/test.pir" ;;
   output_string chan (print_as_program test_file) ;;
   close_out chan
 .
