printing/test.pir
@@ -1,0 +1,1 @@
+(program 1.1.0 (let (nonrec) (termbind (strict) (vardecl x (con integer)) (error con integer)) [[(builtin equalsInteger) [[(builtin addInteger) (con integer) (10)] x]] (con integer) (5)]))
